---
about_this_resource_text: '<p><strong>Instructor:</strong> John Tsitsiklis</p>'
embedded_media:
  - id: Video-YouTube-Stream
    media_location: cCmWW7Hu43A
    parent_uid: 3684c6c16c7389128dbf09aa92a74ca1
    title: Video-YouTube-Stream
    type: Video
    uid: d90746cc9e3d6e2b6e3f3ffaebab5762
  - id: Thumbnail-YouTube-JPG
    media_location: 'https://img.youtube.com/vi/cCmWW7Hu43A/default.jpg'
    parent_uid: 3684c6c16c7389128dbf09aa92a74ca1
    title: Thumbnail-YouTube-JPG
    type: Thumbnail
    uid: f5347e100babff8b1b9aa8952d7bca1c
  - id: 3Play-3PlayYouTubeid-MP4
    media_location: cCmWW7Hu43A
    parent_uid: 3684c6c16c7389128dbf09aa92a74ca1
    title: 3Play-3Play YouTube id
    type: 3Play
    uid: 80fecc10b819d9a8d00566279410f705
  - id: cCmWW7Hu43A.srt
    parent_uid: 3684c6c16c7389128dbf09aa92a74ca1
    technical_location: >-
      https://ocw.mit.edu/resources/res-6-012-introduction-to-probability-spring-2018/part-i-the-fundamentals/the-geometric-series/cCmWW7Hu43A.srt
    title: 3play caption file
    type: null
    uid: f3a1ba22287da515e5c7e86f683561f4
  - id: cCmWW7Hu43A.pdf
    parent_uid: 3684c6c16c7389128dbf09aa92a74ca1
    technical_location: >-
      https://ocw.mit.edu/resources/res-6-012-introduction-to-probability-spring-2018/part-i-the-fundamentals/the-geometric-series/cCmWW7Hu43A.pdf
    title: 3play pdf file
    type: null
    uid: 1f5ebd4ee880f80b369441e5282d9e4a
  - id: Caption-3Play YouTube id-SRT
    parent_uid: 3684c6c16c7389128dbf09aa92a74ca1
    title: Caption-3Play YouTube id-SRT-English - US
    type: Caption
    uid: 8fb8611eecd0ba72e7818db58684e059
  - id: Transcript-3Play YouTube id-PDF
    parent_uid: 3684c6c16c7389128dbf09aa92a74ca1
    title: Transcript-3Play YouTube id-PDF-English - US
    type: Transcript
    uid: b7644dad744440b499eeac8dcddabb42
  - id: Video-InternetArchive-MP4
    media_location: >-
      https://archive.org/download/MITRES.6-012S18/MITRES6_012S18_S01-06_300k.mp4
    parent_uid: 3684c6c16c7389128dbf09aa92a74ca1
    title: Video-Internet Archive-MP4
    type: Video
    uid: 009de778dc8ed22288015a03bdfde295
inline_embed_id: 4719628thegeometricseries6122724
order_index: 177
parent_uid: 9ca6b310dc93095c9ac0f0e5f95e6930
related_resources_text: ''
short_url: the-geometric-series
technical_location: >-
  https://ocw.mit.edu/resources/res-6-012-introduction-to-probability-spring-2018/part-i-the-fundamentals/the-geometric-series
title: The Geometric Series
transcript: >-
  <p><span m="1460">One particular series that shows up in many
  applications,</span> <span m="4710">examples, or problems is the geometric
  series.</span></p><p><span m="7900">[In] the geometric series, we are given a
  certain number,</span> <span m="10590">alpha, and we want to sum all the
  powers of alpha, starting</span> <span m="15130">from the 0th power, which is
  equal to 1, the first power,</span> <span m="18660">and so on, and this gives
  us an infinite series.</span></p><p><span m="21690">It's the sum of alpha to
  the i where i</span> <span m="24030">ranges from 0 to
  infinity.</span></p><p><span m="26490">Now, for this series to converge, we
  need subsequent</span> <span m="29610">terms, the different terms in the
  series, to become smaller</span> <span m="32910">and
  smaller.</span></p><p><span m="33900">And for this reason, we're going to make
  the assumption</span> <span m="36280">that the number alpha is less than 1 in
  magnitude, which</span> <span m="40430">implies that consecutive terms go to
  zero.</span></p><p><span m="45100">Let us introduce some
  notation.</span></p><p><span m="46740">Let us denote the infinite sum by s,
  and we're going to use</span> <span m="50620">that notation
  shortly.</span></p><p><span m="52700">One way of evaluating this series is to
  start from an</span> <span m="56280">algebraic identity, namely the
  following.</span></p><p><span m="59870">Let us take 1 minus alpha and multiply
  it by the terms in</span> <span m="65180">the series, but going only up to the
  term alpha to the n.</span></p><p><span m="71220">So it's a finite
  series.</span></p><p><span m="73780">We do this multiplication, we get a bunch
  of terms, we do</span> <span m="77190">the cancellations, and what is left at
  the end is 1 minus</span> <span m="82230">alpha to the power n plus
  1.</span></p><p><span m="85450">What we do next is we take the limit as n goes
  to infinity.</span></p><p><span m="90970">On the left hand side, we have the
  term 1 minus alpha, and</span> <span m="95759">then the limit of this finite
  series is by definition the</span> <span m="99600">infinite series, which
  we're denoting by s.</span></p><p><span m="102789">On the right hand side, we
  have the term 1.</span></p><p><span m="106250">How about this
  term?</span></p><p><span m="107870">Since alpha is less than 1 in magnitude,
  this converges to 0</span> <span m="111950">as alpha goes to infinity, so that
  term disappears.</span></p><p><span m="115830">We can now solve this relation,
  and we obtain that s</span> <span m="119090">is equal to 1 over 1 minus alpha,
  and this is the formula</span> <span m="123530">for the infinite geometric
  series.</span></p><p><span m="126450">There's another way of deriving the same
  result,</span> <span m="129220">which is interesting, so let us go through it
  as well.</span></p><p><span m="133770">The infinite geometric series has one
  first term and then</span> <span m="139680">the remaining terms, which is a
  sum for i going from 1 to</span> <span m="144620">infinity of alpha to the
  i.</span></p><p><span m="147860">Now, we can take a factor of alpha out of
  this infinite sum</span> <span m="152200">and write it as 1 plus alpha, the
  sum of alpha to the i, but</span> <span m="158680">because we took out one
  factor of alpha, here, we're going to</span> <span m="163180">have smaller
  powers.</span></p><p><span m="164400">So now the sum starts from 0 and goes up
  to infinity.</span></p><p><span m="172480">Now, this is just 1 plus alpha
  times s because here, we have</span> <span m="178220">the infinite geometric
  series.</span></p><p><span m="180920">Therefore, if we subtract alpha s from
  both sides of</span> <span m="185620">this equality, we get s times 1 minus
  alpha equal to 1.</span></p><p><span m="192590">And now by moving 1 minus
  alpha to the denominator, we</span> <span m="196120">get again the same
  expression.</span></p><p><span m="198770">So this is an alternative way of
  deriving the same result.</span></p><p><span m="201510">However, there's one
  word of caution.</span></p><p><span m="203690">In this step, we subtracted
  alpha s from both</span> <span m="207990">sides of the
  equation.</span></p><p><span m="210230">And in order to do that, this is only
  possible if we take</span> <span m="215170">for granted that s is a finite
  number.</span></p><p><span m="220240">So this is taken for granted in order to
  carry out this</span> <span m="225990">derivation.</span></p><p><span
  m="227280">This is to be contrasted with the first derivation, in which</span>
  <span m="231050">we didn't have to make any such
  assumption.</span></p><p><span m="233690">So strictly speaking, for this
  derivation here to be correct,</span> <span m="237340">we need to have some
  independent way of verifying</span> <span m="239890">that s is less than
  infinity.</span></p><p><span m="242200">But other than that, it's an
  interesting algebraic trick.</span></p><p>&nbsp;</p>
uid: 3684c6c16c7389128dbf09aa92a74ca1
type: courses
layout: video
---
