---
about_this_resource_text: '<p><strong>Instructor:</strong> Dr. Peter Dourmashkin</p>'
embedded_media:
  - id: Video-YouTube-Stream
    media_location: flwYlUfw4WU
    parent_uid: ff0f5300ad954089c6ef61a1709b4f98
    title: Video-YouTube-Stream
    type: Video
    uid: 489e5b404b4eeb0508c274487f901566
  - id: Thumbnail-YouTube-JPG
    media_location: 'https://img.youtube.com/vi/flwYlUfw4WU/default.jpg'
    parent_uid: ff0f5300ad954089c6ef61a1709b4f98
    title: Thumbnail-YouTube-JPG
    type: Thumbnail
    uid: ea4b2c60beed631391eadf81c1f0f203
  - id: 3Play-3PlayYouTubeid-MP4
    media_location: flwYlUfw4WU
    parent_uid: ff0f5300ad954089c6ef61a1709b4f98
    title: 3Play-3Play YouTube id
    type: 3Play
    uid: 128282b2d0859301630c2924a8bb17a2
  - id: Video-iTunesU-MP4
    media_location: 'https://itunes.apple.com/us/itunes-u/id1223579658'
    parent_uid: ff0f5300ad954089c6ef61a1709b4f98
    title: Video-iTunes U-MP4
    type: Video
    uid: ca03ca06326b4c080135c56579bd7b35
  - id: Video-InternetArchive-MP4
    media_location: 'https://archive.org/download/MIT8.01F16/MIT8_01F16_L14v03_360p.mp4'
    parent_uid: ff0f5300ad954089c6ef61a1709b4f98
    title: Video-Internet Archive-MP4
    type: Video
    uid: bd3a989736ec132f149f5a121a7d23e9
  - id: flwYlUfw4WU.srt
    parent_uid: ff0f5300ad954089c6ef61a1709b4f98
    technical_location: >-
      https://ocw.mit.edu/courses/physics/8-01sc-classical-mechanics-fall-2016/week-4-drag-forces-constraints-and-continuous-systems/14.3-resistive-forces-high-speed-case/14.3-resistive-forces-high-speed-case/flwYlUfw4WU.srt
    title: 3play caption file
    type: null
    uid: 9f5d33d0dd0f64dfd0362b42a37806a6
  - id: flwYlUfw4WU.pdf
    parent_uid: ff0f5300ad954089c6ef61a1709b4f98
    technical_location: >-
      https://ocw.mit.edu/courses/physics/8-01sc-classical-mechanics-fall-2016/week-4-drag-forces-constraints-and-continuous-systems/14.3-resistive-forces-high-speed-case/14.3-resistive-forces-high-speed-case/flwYlUfw4WU.pdf
    title: 3play pdf file
    type: null
    uid: 59d1a40fe045f1c14f9e020360ee0fe7
  - id: Caption-3Play YouTube id-SRT
    parent_uid: ff0f5300ad954089c6ef61a1709b4f98
    title: Caption-3Play YouTube id-SRT-English - US
    type: Caption
    uid: 7516f98f82803e28b97d1f4811f89051
  - id: Transcript-3Play YouTube id-PDF
    parent_uid: ff0f5300ad954089c6ef61a1709b4f98
    title: Transcript-3Play YouTube id-PDF-English - US
    type: Transcript
    uid: bf7fdc02cff2ce86553a0df14c36fa97
inline_embed_id: 2826546914.3resistiveforceshighspeedcase57663711
order_index: 963
parent_uid: cc32eace0df413671aa69a03a79b0c59
related_resources_text: ''
short_url: 14.3-resistive-forces-high-speed-case
technical_location: >-
  https://ocw.mit.edu/courses/physics/8-01sc-classical-mechanics-fall-2016/week-4-drag-forces-constraints-and-continuous-systems/14.3-resistive-forces-high-speed-case/14.3-resistive-forces-high-speed-case
title: 14.3 Resistive Forces - High Speed Case
transcript: >-
  <p><span m='3020'>Now we're going to analyze a more complicated example</span>
  <span m='6050'>of drag forces, where we have an object falling</span> <span
  m='10630'>in a gravitational field with gravity.</span> </p><p><span
  m='12450'>We have a resistive force.</span> </p><p><span m='15230'>And this is
  an object in air.</span> </p><p><span m='17570'>And so our model will be for
  the resistive force</span> <span m='21840'>that it's going to be proportional
  to the velocity</span> <span m='24380'>squared.</span> </p><p><span
  m='25480'>Now to get its direction right, opposing the motion, j hat.</span>
  </p><p><span m='29760'>So this will turn out to be a more complicated
  analysis.</span> </p><p><span m='33460'>But first again, let's think about the
  units</span> <span m='35780'>of our coefficient beta.</span> </p><p><span
  m='37510'>It has the units of force divided by velocity squared.</span>
  </p><p><span m='41380'>So we write the units of force, kilogram meters</span>
  <span m='44580'>per second squared, and the units</span> <span m='46660'>of
  velocity squared, meter squared per second squared.</span> </p><p><span
  m='51860'>And so we see that we have units of kilogram per meter</span> <span
  m='57100'>for our coefficient beta.</span> </p><p><span m='59080'>Now, we'll
  apply as usual Newton's second law,</span> <span m='63300'>F equals m a, to
  get our equation of motion.</span> </p><p><span m='66330'>We're looking at the
  j direction.</span> </p><p><span m='68110'>And our forces are gravity minus
  the velocity</span> <span m='72110'>squared resistive drag force.</span>
  </p><p><span m='74650'>And that's equal to the derivative of the
  velocity</span> <span m='77630'>dv/dt.</span> </p><p><span m='78670'>In this
  example, it's a one dimensional motion.</span> </p><p><span m='80960'>So I'm
  dropping any mention of y direction for simplicity.</span> </p><p><span
  m='85970'>Now we can rewrite this equation as dv/dt.</span> </p><p><span
  m='90120'>Let's divide through by m is g minus beta over m v square.</span>
  </p><p><span m='96840'>And this is a linear-- it's a first order
  differential</span> <span m='103550'>equation, dv/dt.</span> </p><p><span
  m='105820'>It's a non-linear equation because the velocity</span> <span
  m='109320'>term appears here as a square and there's a constant term.</span>
  </p><p><span m='113240'>But we can still apply our technique</span> <span
  m='114810'>of separation of variables.</span> </p><p><span m='116670'>And so
  when we write this equation as dv/dt</span> <span m='122380'>we'll separate
  out dv's and t's, so we have d d times</span> <span m='128300'>g minus beta
  over and m v squared is equal to dt.</span> </p><p><span m='134820'>Now, I'm
  going to do two things just to clean this up</span> <span m='137280'>for
  algebra a little bit later.</span> </p><p><span m='139160'>I'm going to
  multiply both sides by a minus sign.</span> </p><p><span m='142870'>And I'm
  going to pull the g out.</span> </p><p><span m='146310'>So I have 1 minus beta
  over m g v squared.</span> </p><p><span m='152930'>And on the other side, I
  have minus dt.</span> </p><p><span m='158820'>And now I can get this equation
  in the form</span> <span m='162310'>that I'd like to integrate, which</span>
  <span m='163840'>is minus dv times 1 minus beta over m g v squared
  equals</span> <span m='171510'>minus gdt.</span> </p><p><span m='174840'>Now,
  the trouble here is this integral is a little bit</span> <span
  m='177610'>complicated.</span> </p><p><span m='178329'>So I'd like to make a
  change of variable.</span> </p><p><span m='180660'>And my change of variable
  will be</span> <span m='182350'>u equals the square root of beta m g times v.
  And that implies</span> <span m='189990'>that du is beta m g dv.</span>
  </p><p><span m='196290'>And the limits, if we start our object at rest,</span>
  <span m='199680'>so if u0 equals 0, then because v0 equal 0,</span> <span
  m='207980'>that's our first limit.</span> </p><p><span m='210570'>Now we have
  to be a little bit careful</span> <span m='212450'>because if we drop this
  object at rest, initially</span> <span m='215320'>it will be moving very
  slowly.</span> </p><p><span m='217570'>And so our resistive model doesn't
  actually apply.</span> </p><p><span m='221390'>However, we're going to neglect
  that effect even</span> <span m='224534'>though if we were to do a more
  complicated analysis,</span> <span m='226700'>we would have to change our
  model as the object is</span> <span m='229430'>following, so it would be a
  multi-stage motion.</span> </p><p><span m='231829'>First, at the beginning
  with our only velocity</span> <span m='234730'>dependent resistant.</span>
  </p><p><span m='235829'>And then as it gets some initial speed and it's going
  faster,</span> <span m='239579'>we change our model.</span> </p><p><span
  m='240460'>That's why the actual problem can be quite complicated.</span>
  </p><p><span m='243350'>But we're just trying to keep things simple
  here.</span> </p><p><span m='245670'>And then u of t is square root of beta mg
  d of t.</span> </p><p><span m='252510'>And then with this change of variable,
  my integration,</span> <span m='256180'>remember I have a dv, so I have to
  multiply the left side by mg</span> <span m='263090'>over beta.</span>
  </p><p><span m='264430'>And I'm integrating with a minus sign du times
  1</span> <span m='269000'>minus u squared from 0 to this final value u of
  t</span> <span m='275680'>And over here I'm just integrating minus g
  dt.</span> </p><p><span m='284690'>Now again, for simplicity, I'm going</span>
  <span m='288590'>to bring this term, the beta over mg over to the other
  side.</span> </p><p><span m='293960'>So I'll use the magic of our light
  board</span> <span m='298900'>by just erasing that and bringing it</span>
  <span m='302010'>to the other side, which makes my life a little
  easier.</span> </p><p><span m='305830'>And now, this interval can be done by
  the method</span> <span m='310130'>of integration by parts.</span>
  </p><p><span m='311710'>It's a nice problem in calculus.</span> </p><p><span
  m='314070'>And you can verify for yourself that the result</span> <span
  m='317790'>is one half natural log of 1 plus u over 1</span> <span
  m='323390'>minus u evaluated at our limits.</span> </p><p><span m='328380'>And
  over here I have minus g square root of beta over mg.</span> </p><p><span
  m='335720'>Now, once again, for a little bit of simplicity,</span> <span
  m='339220'>I'm going to bring the 2 over to the other side.</span>
  </p><p><span m='345090'>And now, I evaluate my limits.</span> </p><p><span
  m='347720'>Now recall that when you have a minus log,</span> <span
  m='351930'>we're flipping, because log of b over a equals minus</span> <span
  m='356000'>log over ab, so when I put out my limits in,</span> <span
  m='359210'>I have natural log of-- now remember, what are our limits?</span>
  </p><p><span m='363430'>We have 1-- I'm flipping-- minus u is beta mg times v
  of t.</span> </p><p><span m='375080'>And I have the 1 plus beta mg v of
  t.</span> </p><p><span m='385060'>And that's equal to minus as 2g square root
  of beta mg.</span> </p><p><span m='391040'>Now, again, we'll use the fact that
  e to log of x is x.</span> </p><p><span m='397090'>And so if I exponentiate
  both sides,</span> <span m='399500'>I end up with 1 minus the square root of
  beta mg d of t over 1</span> <span m='407210'>plus square root of beta mg v of
  t</span> <span m='411730'>is equal to exponential minus 2g beta mg times
  t.</span> </p><p><span m='419940'>And we'll just move that.</span>
  </p><p><span m='422890'>OK, now this is a little bit of algebra.</span>
  </p><p><span m='425050'>I want to solve for v of t.</span> </p><p><span
  m='427510'>If I bring this side over to there,</span> <span m='430250'>I'll
  just do that to make the first step a little simpler</span> <span
  m='432790'>to see.</span> </p><p><span m='433610'>So we have 1 minus square
  root of beta mg v of t</span> <span m='439680'>equals 1 plus square root of
  beta over mg v of t times</span> <span m='447383'>e to the minus this factor
  2g square root of beta mg t.</span> </p><p><span m='455270'>Now this is a lot
  of stuff to carry around.</span> </p><p><span m='458860'>I'd like to introduce
  a constant here,</span> <span m='462210'>tao, which I'm going to find to be
  square root of mg beta 1</span> <span m='469159'>over 2g.</span> </p><p><span
  m='471190'>And so this whole term is going to just be e to the minus
  tao.</span> </p><p><span m='477740'>It's a nice example for you to work out
  that the units of tao</span> <span m='482950'>are the units of seconds.</span>
  </p><p><span m='485270'>And that's a little exercise to work out.</span>
  </p><p><span m='487780'>Now, I just have to collect my terms.</span>
  </p><p><span m='490840'>And what I'll do is I'll collect the T</span> <span
  m='495770'>terms on the right and the terms that don't have vt on the
  left.</span> </p><p><span m='501510'>So I have 1 minus e to the minus t over
  tao</span> <span m='506470'>on the left is equal to 1 plus e to the minus t
  over tao</span> <span m='512679'>on the right times beta mg v of t.</span>
  </p><p><span m='520140'>And so I get my solution, v of t equals</span> <span
  m='524330'>the square root of mg over beta times 1 minus</span> <span
  m='529940'>e to the minus t over tau over 1 plus e to the minus t over
  tao.</span> </p><p><span m='537970'>Well, it's not a simple solution at
  all.</span> </p><p><span m='543150'>But let's examine when you have a case
  like this-- again,</span> <span m='546860'>it would be a nice exercise to
  graph this out.</span> </p><p><span m='550380'>But right now we're going to
  consider the limit</span> <span m='553190'>as t goes to infinity.</span>
  </p><p><span m='555470'>And remember that e minus t over t</span> <span
  m='558730'>goes to 0 when t goes to infinity.</span> </p><p><span
  m='561690'>So we just have 1 over 1.</span> </p><p><span m='564480'>And what
  we get as t goes to infinity</span> <span m='567800'>is the quantity mg over
  beta.</span> </p><p><span m='571430'>And this is what we call the terminal
  velocity.</span> </p><p><span m='576320'>Now what does terminal velocity
  mean?</span> </p><p><span m='578510'>Well, when object is falling and there's
  a resistive force,</span> <span m='581640'>as the object falls faster and
  faster,</span> <span m='584130'>the resistive force gets greater and
  greater</span> <span m='586410'>until if we go back to Newton's second law and
  look at it,</span> <span m='590200'>as v gets faster and faster,
  eventually</span> <span m='593610'>these two terms are equal.</span>
  </p><p><span m='596220'>And when these two terms are equal,</span> <span
  m='598020'>that's the statement that the right-hand side has to be
  zero.</span> </p><p><span m='602180'>So what we mean by terminal
  velocity</span> <span m='604820'>is it's the velocity is no longer changing in
  time.</span> </p><p><span m='608690'>And then we can immediately check our
  work</span> <span m='611250'>by going to Newton's second law and see
  what</span> <span m='613970'>that case is if we set this quantity equal to
  zero.</span> </p><p><span m='617970'>In other words, when we set mg minus beta
  v</span> <span m='622820'>squared terminal equal to 0 we can solve for v
  terminal,</span> <span m='631420'>and we get a square root of mg divided by
  beta.</span> </p><p><span m='636290'>And that agrees with our lengthy
  calculation.</span> </p><p><span m='641870'>So we think we're on the right
  track.</span> </p><p></p>
uid: ff0f5300ad954089c6ef61a1709b4f98
type: courses
layout: video
---
